immutable buffers library

examples/low-mitls-experiments/ImmutableBuffer.fst
@@ -6,67 +6,56 @@ module HST = FStar.HyperStack.ST
 module Seq = FStar.Seq
 module U32 = FStar.UInt32
 
-// private let crel (a:Type0) :B.srel a = fun s1 s2 -> Seq.equal s1 s2
+module IB = LowStar.ImmutableBuffer
 
-// private let cpred (#a:Type0) (s:Seq.seq a) :B.spred a = fun s1 -> Seq.equal s1 s
 
-// type immutable_buffer (a:Type0) = B.mbuffer a (crel a) (crel a)
+(*
+ * Testing normalization of lists in the buffer library
+ *)
+[@"opaque_to_smt"]
+let l :list int = [1; 2; 3; 4; 5; 6; 7; 8; 9; 10]
 
-// let gsub (#a:Type0) (b:immutable_buffer a) (i:U32.t) (len:U32.t)
-//   :Ghost (immutable_buffer a) (requires (U32.v i + U32.v len <= B.length b)) (ensures (fun _ -> True))
-//   = B.mgsub b i len (crel a)
+let test2 (lll:list int{List.Tot.length lll > 0 /\
+                      List.Tot.length lll <= UInt.max_int 32})
+  :HST.ST unit (fun h0 -> HS.is_stack_region (HS.get_tip h0)) (fun _ _ _ -> True)=
+  let b = B.gcmalloc_of_list HS.root l in
+  assert (B.length b == 10);
+  let h = HST.get () in
+  assert (B.as_seq h b == Seq.seq_of_list l);
+  assert (B.length b == List.Tot.length l);
+  let ll = [1;2;3;4;5;6;7;8;9;10;11] in
+  HST.push_frame ();
+  let b = B.alloca_of_list ll in
+  assert (B.length b == 11);
+  let h = HST.get () in
+  assert (B.as_seq h b == Seq.seq_of_list ll);
+  assert (B.length b == List.Tot.length ll);
+  let b = B.alloca_of_list lll in
+  let h = HST.get () in
+  assert (B.as_seq h b == Seq.seq_of_list lll);
+  assert (B.length b == List.Tot.length lll);
+  HST.pop_frame ()
 
-// let sub (#a:Type0) (b:immutable_buffer a) (i:U32.t) (len:U32.t)
-//   :HST.Stack (immutable_buffer a)
-//              (requires (fun h -> U32.v i + U32.v len <= B.length b /\ B.live h b))
-//              (ensures  (fun h y h' -> h == h' /\ y == gsub b i len))
-//   = B.msub b i len (crel a)
+assume val havoc (#a:Type0) (#rrel #rel:B.srel a) (b:B.mbuffer a rrel rel) :HST.St unit
 
-// let offset (#a:Type0) (b:immutable_buffer a) (i:U32.t)
-//   :HST.Stack (immutable_buffer a)
-//              (requires (fun h -> U32.v i <= B.length b /\ B.live h b))
-//              (ensures  (fun h y h' -> h == h' /\ y == gsub b i (U32.sub (B.len b) i)))
-//   = B.moffset b i (crel a)
-
-// let gcmalloc_of_list (#a:Type0) (r:HS.rid) (init:list a)
-//   :HST.ST (b:immutable_buffer a {
-//     let len = FStar.List.Tot.length init in
-//     B.recallable b /\
-//     B.alloc_post_static r len b /\
-//     B.alloc_of_list_post len b
-//   })
-//           (requires (fun h -> HST.is_eternal_region r /\ B.gcmalloc_of_list_pre #a init))
-//           (ensures  (fun h b h' -> let len = FStar.List.Tot.length init in
-//                                  B.alloc_post_common r len b h h' /\
-//                                  B.as_seq h' b == Seq.seq_of_list init /\
-// 				 B.witnessed b (cpred (Seq.seq_of_list init))))
-//   = let b = B.mgcmalloc_of_list r init in
-//     B.witness_p b (cpred (Seq.seq_of_list init));
-//     b
-
-// let recall_contents (#a:Type0) (b:immutable_buffer a) (s:Seq.seq a)
-//   :HST.ST unit (requires (fun _       -> B.witnessed b (cpred s)))
-//                (ensures  (fun h0 _ h1 -> h0 == h1 /\ Seq.equal (B.as_seq h0 b) s))
-//   = B.recall_p b (cpred s)
-
-// assume val havoc (#a:Type0) (#rrel #rel:B.srel a) (b:B.mbuffer a rrel rel) :HST.St unit
-
-// let test (l:list int{List.Tot.length l == 10}) :HST.St unit =
-//   let ls = Seq.seq_of_list l in
-//   let b =  gcmalloc_of_list HS.root l in
-
-//   havoc b;
-//   B.recall b;
-//   recall_contents b ls;
-//   let h = HST.get () in
-//   assert (B.as_seq h b == ls);
+let test (l:list int{List.Tot.length l == 10}) :HST.St unit =
+  let ls = Seq.seq_of_list l in
+  let b =  IB.igcmalloc_of_list HS.root l in
+  assert (B.length b == 10);
+  havoc b;
+  IB.recall_contents b ls;
+  let h = HST.get () in
+  assert (B.as_seq h b == ls);
+  assert (B.live h b);
   
-//   let sb = sub b 0ul 2ul in
-//   havoc sb;
-//   B.recall b;
-//   recall_contents b ls;  
-//   let h = HST.get () in
-//   assert (B.as_seq h b == ls)
+  let sb = IB.isub b 0ul 2ul in
+  IB.witness_contents sb (Seq.slice ls 0 2);
+  havoc sb;
+  IB.recall_contents sb (Seq.slice ls 0 2);
+  IB.recall_contents b ls;
+  let h = HST.get () in
+  assert (B.as_seq h b == ls);
+  assert (B.as_seq h sb = Seq.slice ls 0 2)
 
 
 // (*
@@ -101,31 +90,3 @@ module U32 = FStar.UInt32
 //     B.recall_p bb (cpred s);
 //     let h = HST.get () in
 //     assert (B.as_seq h bb == s)
-
-
-(*
- * Testing normalization of lists in the buffer library
- *)
-[@"opaque_to_smt"]
-let l :list int = [1; 2; 3; 4; 5; 6; 7; 8; 9; 10]
-
-let test2 (lll:list int{List.Tot.length lll > 0 /\
-                      List.Tot.length lll <= UInt.max_int 32})
-  :HST.ST unit (fun h0 -> HS.is_stack_region (HS.get_tip h0)) (fun _ _ _ -> True)=
-  let b = B.gcmalloc_of_list HS.root l in
-  assert (B.length b == 10);
-  let h = HST.get () in
-  assert (B.as_seq h b == Seq.seq_of_list l);
-  assert (B.length b == List.Tot.length l);
-  let ll = [1;2;3;4;5;6;7;8;9;10;11] in
-  HST.push_frame ();
-  let b = B.alloca_of_list ll in
-  assert (B.length b == 11);
-  let h = HST.get () in
-  assert (B.as_seq h b == Seq.seq_of_list ll);
-  assert (B.length b == List.Tot.length ll);
-  let b = B.alloca_of_list lll in
-  let h = HST.get () in
-  assert (B.as_seq h b == Seq.seq_of_list lll);
-  assert (B.length b == List.Tot.length lll);
-  HST.pop_frame ()
